add completeness

VmProofs.v
@@ -23,8 +23,11 @@ Proof.
   (* H = fuel ok, interpret_all' program state fuel = Ok output_state *)
   - compute in H; discriminate.
   - unfold interpret_all' in H |- *; fold interpret_all' in H |- *.
-    destruct (List.nth_error program (pc state)) as [instr|]; [|discriminate].
-    destruct instr; (destruct (interpret _ state); [apply IHfuel; exact H | discriminate]) || exact H.
+    destruct (List.nth_error program (pc state)) as [instr|] eqn:H_instr_is.
+    destruct state.(halted).
+    + exact H.
+    + destruct instr; (destruct (interpret _ state); [apply IHfuel; exact H | discriminate]) || exact H.
+    + exact H.
 Qed.
 
 Theorem more_fuel_ok:
@@ -83,8 +86,8 @@ Proof.
   unfold succeeds in succeeds_fuel.
   destruct (interpret_all_with_fuel program fuel) as [output_state | err_msg] eqn:fuel_ok.
   - unfold interpret_all_with_fuel in fuel_ok.
-    assert (more_fuel_res : interpret_all' program {| stack := []; pc := 0; memory := NatMap.empty nat |} more_fuel = Ok output_state).
-    apply (more_fuel_ok program {| stack := []; pc := 0; memory := NatMap.empty nat |} output_state fuel more_fuel more_fuel_ge_fuel fuel_ok).
+    assert (more_fuel_res : interpret_all' program {| stack := []; pc := 0; memory := NatMap.empty nat; halted := false |} more_fuel = Ok output_state).
+    apply (more_fuel_ok program {| stack := []; pc := 0; memory := NatMap.empty nat; halted := false |} output_state fuel more_fuel more_fuel_ge_fuel fuel_ok).
     unfold interpret_all_with_fuel.
     rewrite more_fuel_res.
     reflexivity.
@@ -104,56 +107,40 @@ Qed.
   interpret_all eventually hits 'PC out of bounds' unless there's an
   IOutput.
 
-  In other words, all programs must end with 'IOutput'.
+  In other words, all programs must end with 'IOutput' instruction executed.
+  This doesn't mean that IOutput must literally be the last instruction, but
+  only that it must be the last instruction to be executed for a successful
+  program.
 *)
-Definition halts (state : VmState) (instructions : list Instruction) : Prop :=
+Definition has_halted (state : VmState) (instructions : list Instruction) : Prop :=
   exists output,
     state.(stack) = [output] /\
-    List.nth_error instructions (state.(pc) - 1) = Some IOutput.
+    state.(halted) = true /\
+    List.nth_error instructions state.(pc) = Some IOutput.
 
-Ltac solve_halted instruction initial_state interpret_ok IH :=
-  destruct (interpret instruction initial_state) as [next_state|];
-  [ apply IH with (initial_state := next_state); exact interpret_ok
-    | discriminate interpret_ok ].
+(* The given state is terminal for the instructions.
+   So an output state where we advanced by semantics (step) does not exist.
+*)
+Definition terminal (state : VmState) (instructions : list Instruction) : Prop :=
+  forall output_state, ~(step state instructions output_state).
 
-Theorem ok_implies_halted :
-  forall fuel instructions output_state,
-    interpret_all' instructions
-      {| stack := []; pc := 0 ; memory := NatMap.empty nat |} fuel = Ok output_state ->
-      halts output_state instructions.
+
+(* If a program halts, then it is in terminal step. Semantically it is impossible
+  for a program to proceed further.
+*)
+Theorem halted_implies_terminal :
+  forall state program, has_halted state program -> terminal state program.
 Proof.
-  intros fuel.
-  generalize {| stack := []; pc := 0; memory := NatMap.empty nat |} as initial_state.
+  intros state program H_halted.
+  destruct H_halted as [out [H_stack [H_halted H_nth]]].
+  intros output_state H_step.
 
-  induction fuel as [|fuel IH_fuel]; intros initial_state instructions output_state interpret_ok.
-  - discriminate interpret_ok.
-  - simpl in interpret_ok.
-    destruct (nth_error instructions (pc initial_state)) eqn:nth_err.
-    + destruct i.
-      * solve_halted (IPush n) initial_state interpret_ok IH_fuel.
-      * solve_halted IMstore initial_state interpret_ok IH_fuel.
-      * solve_halted IMload initial_state interpret_ok IH_fuel.
-      * solve_halted IAdd initial_state interpret_ok IH_fuel.
-      * destruct initial_state as [stack pc memory].
-        destruct stack as [|a rest]; simpl in interpret_ok.
-        -- discriminate interpret_ok.
-        -- injection interpret_ok as H_output_eq.
-           subst.
-           exists a.
-           split.
-           ++ reflexivity.
-           ++ simpl.
-              assert (pc_eq: pc + 1 - 1 = pc) by lia.
-              rewrite pc_eq.
-              simpl in nth_err.
-              exact nth_err.
-      * solve_halted IEq initial_state interpret_ok IH_fuel.
-      * solve_halted IJmpi initial_state interpret_ok IH_fuel.
-      * solve_halted IDup initial_state interpret_ok IH_fuel.
-      * solve_halted IPop initial_state interpret_ok IH_fuel.
-      * solve_halted ISwap initial_state interpret_ok IH_fuel.
-    + discriminate interpret_ok.
+  inversion H_step; subst; simpl in *; rewrite H in H_nth; try discriminate H_nth.
+  discriminate H_halted.
 Qed.
+
+Definition well_formed_program (instructions: list Instruction) (output_state: VmState) : Prop :=
+  True.
 
 Ltac solve_complete nth_ok H :=
     subst;
@@ -165,8 +152,8 @@ Ltac solve_complete nth_ok H :=
 Theorem interpret_complete :
   forall instructions instruction stack pc memory out_state,
     nth_error instructions pc = Some instruction ->
-    step {| stack := stack; pc := pc; memory := memory |} instructions out_state ->
-    interpret instruction {| stack := stack; pc := pc; memory := memory |} = Ok out_state.
+    step {| stack := stack; pc := pc; memory := memory; halted := false |} instructions out_state ->
+    interpret instruction {| stack := stack; pc := pc; memory := memory; halted := false |} = Ok out_state.
 Proof.
   intros instructions instruction stack pc memory out_state.
   intros nth_ok step_ok.
@@ -209,9 +196,10 @@ Theorem interpret_sound:
     interpret instruction {|
       stack := stack;
       pc := pc;
-      memory := memory
+      memory := memory;
+      halted := false
     |} = Ok output_state ->
-    step {| stack := stack; pc := pc; memory := memory |} instructions output_state.
+    step {| stack := stack; pc := pc; memory := memory; halted := false |} instructions output_state.
 Proof.
   intros instructions instruction stack pc memory output_state.
   intros nth_ok interpret_ok.
@@ -327,8 +315,8 @@ Qed.
 Theorem interpret_correct:
   forall instructions instruction stack pc memory out_state,
     nth_error instructions pc = Some instruction ->
-    step {| stack := stack; pc := pc; memory := memory |} instructions out_state <->
-    interpret instruction {| stack := stack; pc := pc; memory := memory |} = Ok out_state.
+    step {| stack := stack; pc := pc; memory := memory; halted := false |} instructions out_state <->
+    interpret instruction {| stack := stack; pc := pc; memory := memory; halted := false |} = Ok out_state.
 Proof.
   intros.
   split.
@@ -338,15 +326,77 @@ Proof.
     exact H.
 Qed.
 
-(* interpret_all_sound_instruction_case *)
+(* isr = Inversion; Subst; Reflexivity  *)
+Ltac isr H := inversion H; subst; reflexivity.
+
+Theorem interpret_sets_halted_false :
+  forall instruction state output_state,
+    instruction <> IOutput ->
+    interpret instruction state = Ok output_state ->
+    output_state.(halted) = false.
+Proof.
+  intros instruction state output_state H_not_ioutput H_interp_ok.
+  destruct instruction; simpl in H_interp_ok.
+
+  - isr H_interp_ok.
+
+  - destruct (state.(stack)) as [| offset [| value s']].
+    + discriminate.
+    + discriminate.
+    + isr H_interp_ok.
+
+  - destruct state.(stack) as [| offset s'].
+    + discriminate.
+    + destruct (NatMap.find offset state.(memory)).
+      * isr H_interp_ok.
+      * discriminate.
+
+  - destruct (state.(stack)) as [| a [| b s']].
+    + discriminate.
+    + isr H_interp_ok.
+    + isr H_interp_ok.
+
+  - exfalso.
+    apply H_not_ioutput.
+    reflexivity.
+
+  - destruct state.(stack) as [| a [| b s']].
+    + discriminate.
+    + discriminate.
+    + isr H_interp_ok.
+
+  - destruct state.(stack) as [| sj [| addr s']].
+    + discriminate.
+    + discriminate.
+    + destruct (Nat.eqb sj 1).
+      * isr H_interp_ok.
+      * isr H_interp_ok.
+
+  - destruct state.(stack) as [| a s'].
+    + discriminate.
+    + isr H_interp_ok.
+
+  - destruct state.(stack) as [| a s'].
+    + discriminate.
+    + isr H_interp_ok.
+
+  - destruct state.(stack) as [| a [| b s']].
+    + discriminate.
+    + discriminate.
+    + isr H_interp_ok.
+Qed.
+
+(* ia_sic = Interpret_All_Sound_Instruction_Case *)
 Ltac ia_sic
-  instr instructions IH interpret_ok nth_err initial_state output_state :=
+  instr instructions IH interpret_ok nth_err initial_state output_state H_halted :=
   (* sso = single step output state *)
   (* dro = destruct result output *)
   destruct (interpret instr initial_state) as [sso_state|] eqn:dro_eq;
   [ apply (@steps_transitive initial_state sso_state output_state instructions);
-    [ destruct initial_state as [stack pc memory];
-    (* forall instructions instruction stack pc memory output_state *)
+    [ destruct initial_state as [stack pc memory halted];
+      simpl in H_halted;
+      subst halted;
+      (* forall instructions instruction stack pc memory output_state *)
       apply (@interpret_sound instructions instr stack pc memory sso_state);
       [ exact nth_err | exact dro_eq ]
     | apply IH; exact interpret_ok ]
@@ -355,45 +405,151 @@ Ltac ia_sic
 Theorem interpret_all_sound:
   forall fuel instructions output_state,
     interpret_all' instructions
-    {| stack := []; pc := 0; memory := NatMap.empty nat |} fuel = Ok output_state ->
-      steps {| stack := []; pc := 0; memory := NatMap.empty nat |} instructions output_state.
+    {| stack := []; pc := 0; memory := NatMap.empty nat; halted := false |} fuel = Ok output_state ->
+      steps {| stack := []; pc := 0; memory := NatMap.empty nat; halted := false |} instructions output_state.
 Proof.
   intros fuel.
-  (* don't need: remember {| stack := []; pc := 0; memory := NatMap.empty nat |}
-    as initial_state_val eqn:initial_state_eq. *)
-  generalize {| stack := []; pc := 0; memory := NatMap.empty nat |} as initial_state.
+  (*
+    don't need: remember {| stack := []; pc := 0; memory := NatMap.empty nat |}
+    as initial_state_val eqn:initial_state_eq.
+
+    Initial state has to be generalized otherwise it's impossible to apply the IH later on.
+  *)
+  generalize {| stack := []; pc := 0; memory := NatMap.empty nat; halted := false |} as initial_state.
   induction fuel as [|fuel IH_fuel].
   - intros initial_state instructions output_state interpret_ok.
     simpl in interpret_ok.
     discriminate interpret_ok.
   - intros initial_state instructions output_state interpret_ok.
     simpl in interpret_ok.
-    destruct (nth_error instructions (pc initial_state)) as [instr|] eqn:nth_err.
-    + destruct instr.
-      * ia_sic (IPush n) instructions IH_fuel interpret_ok nth_err initial_state output_state.
-      * ia_sic IMstore instructions IH_fuel interpret_ok nth_err initial_state output_state.
-      * ia_sic IMload instructions IH_fuel interpret_ok nth_err initial_state output_state.
-      * ia_sic IAdd instructions IH_fuel interpret_ok nth_err initial_state output_state.
-      * (* Needed because IOutput is separately matched in interpret_all *)
-        destruct initial_state as [stack pc memory].
-        -- destruct stack as [|a others] eqn:stack_destruct.
-          ++ subst.
-            simpl in interpret_ok.
-            discriminate interpret_ok.
-          ++ subst.
-             simpl in interpret_ok, nth_err.
-             injection interpret_ok as H_output_state_eq.
-             subst.
-             apply steps_transitive with (state2 := {| stack := [a]; pc := pc + 1; memory := memory |}).
-             ** apply interpret_sound with (IOutput).
-                --- exact nth_err.
-                --- simpl.
-                    reflexivity.
-             ** apply steps_reflexive.
-      * ia_sic IEq instructions IH_fuel interpret_ok nth_err initial_state output_state.
-      * ia_sic IJmpi instructions IH_fuel interpret_ok nth_err initial_state output_state.
-      * ia_sic IDup instructions IH_fuel interpret_ok nth_err initial_state output_state.
-      * ia_sic IPop instructions IH_fuel interpret_ok nth_err initial_state output_state.
-      * ia_sic ISwap instructions IH_fuel interpret_ok nth_err initial_state output_state.
-    + discriminate interpret_ok.
+    destruct (initial_state.(halted)) eqn:H_halted.
+    + injection interpret_ok as H_eq.
+      subst output_state.
+      apply steps_reflexive.
+    + destruct (nth_error instructions (pc initial_state)) as [instr|] eqn:nth_err.
+      * destruct instr.
+        ** ia_sic (IPush n) instructions IH_fuel interpret_ok nth_err initial_state output_state H_halted.
+        ** ia_sic IMstore instructions IH_fuel interpret_ok nth_err initial_state output_state H_halted.
+        ** ia_sic IMload instructions IH_fuel interpret_ok nth_err initial_state output_state H_halted.
+        ** ia_sic IAdd instructions IH_fuel interpret_ok nth_err initial_state output_state H_halted.
+        ** (* Needed because IOutput is separately matched in interpret_all, which makes the proof a little different *)
+          destruct initial_state as [stack pc memory halted].
+          --- destruct stack as [|a others] eqn:stack_destruct.
+            ++ subst.
+               simpl in interpret_ok.
+               discriminate interpret_ok.
+            ++ subst.
+               simpl in interpret_ok, nth_err, H_halted.
+               subst halted.
+               injection interpret_ok as H_output_state_eq.
+               subst.
+               apply steps_transitive with (state2 := {| stack := [a]; pc := pc; memory := memory; halted := true |}).
+               *** apply interpret_sound with (IOutput).
+                  -- exact nth_err.
+                  -- simpl.
+                      reflexivity.
+               *** apply steps_reflexive.
+        ** ia_sic IEq instructions IH_fuel interpret_ok nth_err initial_state output_state H_halted.
+        ** ia_sic IJmpi instructions IH_fuel interpret_ok nth_err initial_state output_state H_halted.
+        ** ia_sic IDup instructions IH_fuel interpret_ok nth_err initial_state output_state H_halted.
+        ** ia_sic IPop instructions IH_fuel interpret_ok nth_err initial_state output_state H_halted.
+        ** ia_sic ISwap instructions IH_fuel interpret_ok nth_err initial_state output_state H_halted.
+      * discriminate interpret_ok.
+Qed.
+
+Lemma step_means_not_halted:
+  forall state output_state program,
+    step state program output_state -> state.(halted) = false.
+Proof.
+  intros.
+  inversion H; reflexivity.
+Qed.
+
+Lemma halted_execution_keeps_state_same:
+  forall state output_state program,
+    state.(halted) = true ->
+    steps state program output_state ->
+    output_state = state.
+Proof.
+  intros state output_state program H_halt H_steps.
+  inversion H_steps; subst.
+  - reflexivity.
+  - exfalso.
+    pose proof (step_means_not_halted state state2 program H).
+    rewrite H1 in H_halt.
+    discriminate H_halt.
+Qed.
+
+Lemma halted_interpret_ok:
+  forall program state fuel,
+    state.(halted) = true ->
+    interpret_all' program state (S fuel) = Ok state.
+Proof.
+  intros program state fuel H_halt.
+  simpl.
+  rewrite H_halt.
+  reflexivity.
+Qed.
+
+(* rsse = Rewrite H1; Simpl; Subst; Exact H2 *)
+Ltac rsse H1 H2 := rewrite H1; simpl; subst; exact H2.
+
+(*
+  This proof took a much longer time to complete, particularly because I realized
+  late that it's harder to prove IOutput case without assigning a halted state
+  to the VmState. The key idea for the IOutput case is that if a state
+  has halted, then semantically output state must be equal to state.
+*)
+Theorem interpret_all_complete :
+  forall instructions final_state,
+    well_formed_program instructions final_state ->
+    steps {| stack := []; pc := 0 ; memory := NatMap.empty nat; halted := false |} instructions final_state ->
+    has_halted final_state instructions ->
+    exists fuel,
+      interpret_all' instructions
+      {| stack := []; pc := 0 ; memory := NatMap.empty nat; halted := false |} fuel = Ok final_state.
+Proof.
+  intros instructions final_state well_formed steps_ok halts_instrs.
+
+  induction steps_ok as [| s1 s2 s3 instrs IH].
+  - destruct halts_instrs as [out [H1 [H2 H3]]].
+    exists 1.
+    apply halted_interpret_ok.
+    exact H2.
+  - pose proof (IHsteps_ok well_formed halts_instrs) as H_fuel.
+    
+    destruct H_fuel as [fuel_witness H_fuel_eq].
+    exists (S fuel_witness).
+    
+    simpl.
+    destruct s1 as [stack1 pc1 memory1].
+    inversion IH; subst; simpl.
+    + rsse H5 H_fuel_eq.
+    + rsse H5 H_fuel_eq.
+    + rewrite H5.
+      simpl.
+      subst.
+      rewrite H7.
+      exact H_fuel_eq.
+    + rsse H5 H_fuel_eq.
+    + rewrite H5.
+      remember {| stack := [a] ; pc := pc1; memory := memory1; halted := true |} as s2 eqn:H_eq_s2.
+      
+      assert (s3 = s2).
+      apply halted_execution_keeps_state_same with (program := instrs).
+      * rewrite H_eq_s2.
+        reflexivity.
+      * exact steps_ok.
+      * rewrite -> H. reflexivity. 
+    + rsse H5 H_fuel_eq.
+    + rsse H5 H_fuel_eq.
+    + rewrite -> H5.
+      simpl.
+      subst.
+      apply Nat.eqb_neq in H7.
+      rewrite H7.
+      exact H_fuel_eq.
+    + rsse H5 H_fuel_eq.
+    + rsse H5 H_fuel_eq.
+    + rsse H5 H_fuel_eq.
 Qed.
